More typed ops, more simplification

src/goose_lang/lang.v
@@ -151,17 +151,29 @@ Proof. refine (
        intros H. inversion H. done.
 Defined.
 
+Inductive go_operator : Type :=
+(* binary ops *)
+| GoEquals
+| GoLt
+| GoLe
+| GoGt
+| GoGe
+| GoPlus
+| GoSub
+| GoMul
+| GoDiv
+| GoRemainder
+| GoAnd
+| GoOr
+| GoXor
+| GoBitClear
+| GoShiftl
+| GoShiftr.
+
 Inductive go_instruction : Type :=
 | AngelicExit
 
-(* TODO: other operators (Add, Mul, etc.) should be defined this way, so signed
-   v.s. unsigned mul can be done systematically, and add for integers vs add for
-   strings as well. *)
-| GoEquals (t : go.type)
-| GoLt (t : go.type)
-| GoLe (t : go.type)
-| GoGt (t : go.type)
-| GoGe (t : go.type)
+| GoOp (o : go_operator) (t : go.type)
 
 | GoLoad (t : go.type)
 | GoStore (t : go.type)
@@ -570,40 +582,7 @@ Class GoGlobalContext {ext : ffi_syntax} : Type :=
     map updates, etc. *)
 Class GoLocalContext {ext : ffi_syntax} : Type :=
   {
-    (* includes special-case handling, such as comparing slices to nil. *)
-    go_eq_top_level : go.type → val → val → expr;
-    go_lt : go.type → val → val → option bool;
-    go_le : go.type → val → val → option bool;
-
-    global_addr : go_string → loc;
-    functions : go_string → list go.type → func.t;
-    methods : go.type → go_string → func.t;
-    method_set : go.type → gmap go_string go.signature;
-
-    alloc : go.type → val;
-    load : go.type → val;
-    store : go.type → val;
-    go_zero_val : go.type → val;
-
-    struct_field_ref : go.type → go_string → loc → loc;
-    struct_field_get : go.type → go_string → val → expr;
-    struct_field_set : go.type → go_string → val → val → expr;
-
-    (* map index expressions have their own implementation that does not use the
-       `Index` primitive. It's statically (even with type parameters) known
-       whether an index expression is a map index expression or not a map index
-       expression. https://go.dev/ref/spec#Index_expressions *)
-    index (container_type : go.type) (i : Z) (v : val) : expr;
-    index_ref (container_type : go.type) (i : Z) (v : val) : expr;
-    array_index_ref (elem_type : go.type) (i : Z) (l : loc) : loc;
-
-    to_underlying : go.type → go.type;
-    map_empty : val → val;
-    map_lookup : val → val → bool * val;
-    map_insert : val → val → val → val;
-    map_delete : val → val → val;
-    is_map_domain : val → list val → Prop;
-    composite_literal : go.type → val → expr;
+    is_go_step_pure : ∀ (op : go_instruction) (arg : val) (e' : expr), Prop;
   }.
 
 Module chan.
@@ -737,159 +716,6 @@ Notation "e1 || e2" :=
 Local Notation "# x" := (into_val x%go).
 Local Notation "#" := into_val (at level 0).
 
-Definition is_interface_type `{!GoLocalContext} (t : go.type) : bool :=
-  match (to_underlying t) with
-  | go.InterfaceType _ => true
-  | _ => false
-  end.
-
-(* Based on: https://go.dev/ref/spec#General_interfaces *)
-Definition type_set_term_contains {go_ctx : GoLocalContext} t (e : go.type_term) : bool :=
-  match e with
-  | go.TypeTerm t' => bool_decide (t = t')
-  | go.TypeTermUnderlying t' => bool_decide (to_underlying t = t')
-  end.
-
-Definition type_set_elem_contains {go_ctx : GoLocalContext} t (e : go.interface_elem) : bool :=
-  match e with
-  | go.MethodElem m signature => bool_decide (method_set t !! m = Some signature)
-  | go.TypeElem terms => existsb (type_set_term_contains t) terms
-  end.
-
-Definition type_set_elems_contains {go_ctx : GoLocalContext} t (elems : list go.interface_elem) : bool :=
-  forallb (type_set_elem_contains t) elems.
-
-(** Equals [true] iff t is in the type set of t'. *)
-Definition type_set_contains {go_ctx : GoLocalContext} t t' : bool :=
-  match (to_underlying t') with
-  | go.InterfaceType elems => type_set_elems_contains t elems
-  | _ => bool_decide (t = t')
-  end.
-
-Inductive is_go_step_pure `{!GoGlobalContext} `{!GoLocalContext} :
-  ∀ (op : go_instruction) (arg : val) (e' : expr), Prop :=
-| angelic_exit_step : is_go_step_pure AngelicExit #() (GoInstruction AngelicExit #())%E
-| equals_step t v1 v2 :
-  is_go_step_pure (GoEquals t) (v1, v2)%V (go_eq_top_level t v1 v2)
-| lt_step t v1 v2 :
-  is_go_step_pure (GoLt t) (v1, v2)%V
-    (match go_lt t v1 v2 with | Some b => #b | None => Panic "not ordered" end)
-| le_step t v1 v2 :
-  is_go_step_pure (GoLe t) (v1, v2)%V
-    (match go_le t v1 v2 with | Some b => #b | None => Panic "not ordered" end)
-| gt_step t v1 v2 :
-  is_go_step_pure (GoGt t) (v1, v2)%V
-    (match go_lt t v2 v1 with | Some b => #b | None => Panic "not ordered" end)
-| ge_step t v1 v2 :
-  is_go_step_pure (GoGe t) (v1, v2)%V
-    (match go_le t v2 v1 with | Some b => #b | None => Panic "not ordered" end)
-| load_step t arg : is_go_step_pure (GoLoad t) arg (load t arg)
-| store_step t (l : loc) v : is_go_step_pure (GoStore t) (#l, v)%V (store t #l v)
-| alloc_step t : is_go_step_pure (GoAlloc t) #() (alloc t #())%E
-| prealloc_step (l : loc) : is_go_step_pure GoPrealloc #() #l
-| func_resolve_step f targs : is_go_step_pure (FuncResolve f targs) #() #(functions f targs)
-| method_resolve_step t m : is_go_step_pure (MethodResolve t m) #() #(methods t m)
-| interface_make_step dt v :
-  is_go_step_pure (InterfaceMake dt) v #(interface.mk dt v)
-| interface_get_step m i :
-  is_go_step_pure (InterfaceGet m) #i
-    (match i with
-     | interface.nil => Panic "nil dereference in interface call"
-     | interface.mk t v => (GoInstruction (MethodResolve t m) #() v)%E
-     end)
-| type_assert_step t i :
-  is_go_step_pure (TypeAssert t) #i
-    (match i with
-     | interface.nil => Panic "type assert failed"
-     | interface.mk dt v =>
-         if is_interface_type t then
-           (if (type_set_contains dt t) then #i else Panic "type assert failed")
-         else
-           (if decide (t = dt) then v else Panic "type assert failed")
-     end)
-| type_assert2_step t i :
-  is_go_step_pure (TypeAssert2 t) #i
-    (match i with
-     | interface.nil => (#interface.nil, #false)%V
-     | interface.mk dt v =>
-         if is_interface_type t then
-           (if (type_set_contains dt t) then (#i, #true)%V else (#interface.nil, #false)%V)
-         else
-           (if decide (t = dt) then (v, #true)%V else (go_zero_val t, #false)%E)
-     end)
-| global_var_addr_step v : is_go_step_pure (GlobalVarAddr v) #() #(global_addr v)
-| struct_field_ref_step t f l : is_go_step_pure (StructFieldRef t f) #l #(struct_field_ref t f l)
-| struct_field_get_step t f v :
-  is_go_step_pure (StructFieldGet t f) v (struct_field_get t f v)
-| struct_field_set_step t f v vf :
-  is_go_step_pure (StructFieldSet t f) (v, vf) (struct_field_set t f v vf)
-
-| internal_len_slice_step_pure elem_type s :
-  is_go_step_pure (InternalLen (go.SliceType elem_type)) #s #(s.(slice.len))
-| internal_len_array_step_pure elem_type n v :
-  is_go_step_pure (InternalLen (go.ArrayType n elem_type)) v #(W64 n)
-
-| internal_cap_slice_step_pure elem_type s :
-  is_go_step_pure (InternalCap (go.SliceType elem_type)) #s #(s.(slice.cap))
-| internal_dynamic_array_alloc_pure elem_type (n : w64) :
-  is_go_step_pure (InternalDynamicArrayAlloc elem_type) #n
-    (GoInstruction (GoAlloc $ go.ArrayType (sint.Z n) elem_type) #())
-| internal_slice_make_pure p l c :
-  is_go_step_pure InternalMakeSlice (#p, #l, #c) #(slice.mk p l c)
-| slice_array_step_pure n elem_type p low high:
-  is_go_step_pure (Slice (go.ArrayType n elem_type))
-    (#p, (#low, #high))%V
-    (if decide (0 ≤ sint.Z low ≤ sint.Z high ≤ n) then
-       #(slice.mk (array_index_ref elem_type (sint.Z low) p)
-           (word.sub high low) (word.sub (W64 n) low))
-     else Panic "slice bounds out of range")
-| full_slice_array_step_pure n elem_type p low high max :
-  is_go_step_pure (FullSlice (go.ArrayType n elem_type))
-    (#p, (#low, #high, #max))%V
-    (if decide (0 ≤ sint.Z low ≤ sint.Z high ≤ sint.Z max ∧ sint.Z max ≤ n) then
-       #(slice.mk (array_index_ref elem_type (sint.Z low) p)
-           (word.sub high low) (word.sub max low))
-     else Panic "slice bounds out of range")
-| slice_slice_step_pure elem_type s low high :
-  is_go_step_pure (Slice (go.SliceType elem_type))
-    (#s, (#low, #high))%V
-    (if decide (0 ≤ sint.Z low ≤ sint.Z high ≤ sint.Z s.(slice.cap)) then
-       #(slice.mk (array_index_ref elem_type (sint.Z low) s.(slice.ptr))
-           (word.sub high low) (word.sub s.(slice.cap) low))
-     else Panic "slice bounds out of range")
-| full_slice_slice_step_pure elem_type s low high max :
-  is_go_step_pure (FullSlice (go.SliceType elem_type))
-    (#s, (#low, #high, #max))%V
-    (if decide (0 ≤ sint.Z low ≤ sint.Z high ≤ sint.Z max ∧ sint.Z max ≤ sint.Z s.(slice.cap)) then
-       #(slice.mk (array_index_ref elem_type (sint.Z low) s.(slice.ptr))
-           (word.sub high low) (word.sub max low))
-     else Panic "slice bounds out of range")
-| index_ref_step t v (j : w64) : is_go_step_pure (IndexRef t) (v, #j) (index_ref t (sint.Z j) v)
-| index_step t v (j : w64) : is_go_step_pure (Index t) (v, #j) (index t (sint.Z j) v)
-| array_set_step_pure ty V n (l : array.t ty V n) (v : V) (i : w64) :
-  is_go_step_pure ArraySet (#l, (#i, #v))%V #(array.mk ty n (<[sint.nat i := v ]> (array.arr l)))
-| array_length_step_pure l :
-  is_go_step_pure ArrayLength (ArrayV l)
-    (if decide (length l < 2^63) then
-       #(W64 (length l))
-     else (GoInstruction AngelicExit #()))
-| internal_map_lookup_step_pure m k :
-  is_go_step_pure InternalMapLookup (m, k) (let '(ok, v) := map_lookup m k in (v, #ok))
-| internal_map_insert_step_pure m k v :
-  is_go_step_pure InternalMapInsert (m, k, v) (map_insert m k v)
-| internal_map_delete_step_pure m k :
-  is_go_step_pure InternalMapDelete (m, k) (map_delete m k)
-| internal_map_length_step_pure m ks (H : is_map_domain m ks) :
-  is_go_step_pure InternalMapLength m #(W64 (length ks))
-| internal_map_domain_literal_step_pure m ks (H : is_map_domain m ks) :
-  is_go_step_pure InternalMapDomainLiteral m
-    (LiteralValue ((λ v, KeyedElement None $ ElementExpression $ Val v) <$> ks))
-| internal_map_make_step_pure v :
-  is_go_step_pure InternalMapMake v (map_empty v)
-| composite_literal_step t v :
-  is_go_step_pure (CompositeLiteral t) v (composite_literal t v)
-.
-
 Inductive is_go_step `{!GoGlobalContext} `{!GoLocalContext} :
   ∀ (op : go_instruction) (arg : val) (e' : expr) (s s' : gmap go_string bool), Prop :=
 | package_init_check_step s p :
@@ -987,6 +813,8 @@ Global Instance prim_op2_eq_dec : EqDecision prim_op2.
 Proof. solve_decision. Defined.
 Global Instance prim_op_eq_dec ar : EqDecision (prim_op ar).
 Proof. destruct ar; simpl; apply _. Defined.
+Global Instance go_operator_eq_dec : EqDecision go_operator.
+Proof. solve_decision. Qed.
 Global Instance go_instruction_eq_dec : EqDecision go_instruction.
 Proof. solve_decision. Qed.
 
@@ -1005,33 +833,7 @@ Global Instance func_t_inhabited : Inhabited func.t :=
 Global Instance GoGlobalContext_inhabited : Inhabited GoGlobalContext :=
   populate {| into_val := inhabitant |}.
 Global Instance GoLocalContext_inhabited : Inhabited GoLocalContext :=
-  populate
-  {|
-    go_eq_top_level := inhabitant;
-    go_lt := inhabitant;
-    go_le := inhabitant;
-    global_addr := inhabitant;
-    functions := inhabitant;
-    methods := inhabitant;
-    method_set := inhabitant;
-    alloc := inhabitant;
-    load := inhabitant;
-    store := inhabitant;
-    go_zero_val := inhabitant;
-    struct_field_ref := inhabitant;
-    struct_field_get := inhabitant;
-    struct_field_set := inhabitant;
-    index := inhabitant;
-    index_ref := inhabitant;
-    array_index_ref := inhabitant;
-    to_underlying := inhabitant;
-    map_empty := inhabitant;
-    map_lookup := inhabitant;
-    map_insert := inhabitant;
-    map_delete := inhabitant;
-    is_map_domain := inhabitant;
-    composite_literal := inhabitant;
-  |}.
+  populate {| is_go_step_pure := inhabitant; |}.
 Global Instance GoState_inhabited : Inhabited GoState :=
   populate {| go_lctx := inhabitant; package_state := inhabitant |}.
 
